Semantic/ModalCapybara/Syntax/Exp.lean
@@ -11,7 +11,7 @@ inductive Exp : Sig -> Type where
 | var : Var .var s -> Exp s
 | abs : CaptureSet s -> Ty .capt s -> Exp (s,x) -> Exp s
 | tabs : CaptureSet s -> PureTy s -> Exp (s,X) -> Exp s
-| cabs : CaptureSet s -> Mutability -> Exp (s,C) -> Exp s
+| cabs : CaptureSet s -> CaptureBound s -> Exp (s,C) -> Exp s
 | boxed : CaptureSet s -> SepCtx s -> Exp s -> Exp s
 | reader : Var .var s -> Exp s
 | pack : CaptureSet s -> Var .var s -> Exp s
@@ -34,7 +34,7 @@ def Exp.rename : Exp s1 -> Rename s1 s2 -> Exp s2
 | .var x, f => .var (x.rename f)
 | .abs cs T e, f => .abs (cs.rename f) (T.rename f) (e.rename (f.lift))
 | .tabs cs T e, f => .tabs (cs.rename f) (T.rename f) (e.rename (f.lift))
-| .cabs cs m e, f => .cabs (cs.rename f) m (e.rename (f.lift))
+| .cabs cs cb e, f => .cabs (cs.rename f) (cb.rename f) (e.rename (f.lift))
 | .boxed cs Ψ e, f => .boxed (cs.rename f) (Ψ.rename f) (e.rename f)
 | .reader x, f => .reader (x.rename f)
 | .pack cs x, f => .pack (cs.rename f) (x.rename f)
@@ -100,7 +100,7 @@ def Exp.rename_id {e : Exp s} : e.rename (Rename.id) = e := by
   induction e
   all_goals
     simp [Exp.rename, Ty.rename_id, PureTy.rename_id, Var.rename_id,
-      CaptureSet.rename_id, SepCtx.rename_id, Rename.lift_id, *]
+      CaptureSet.rename_id, CaptureBound.rename_id, SepCtx.rename_id, Rename.lift_id, *]
 
 /-- Renaming distributes over composition of renamings. -/
 theorem Var.rename_comp {x : Var k s1} {f : Rename s1 s2} {g : Rename s2 s3} :
@@ -113,7 +113,7 @@ theorem Exp.rename_comp {e : Exp s1} {f : Rename s1 s2} {g : Rename s2 s3} :
   induction e generalizing s2 s3
   all_goals
     simp [Exp.rename, Ty.rename_comp, PureTy.rename_comp, Var.rename_comp,
-      CaptureSet.rename_comp, SepCtx.rename_comp, Rename.lift_comp, *]
+      CaptureSet.rename_comp, CaptureBound.rename_comp, SepCtx.rename_comp, Rename.lift_comp, *]
 
 /-- Weakening commutes with renaming under a binder. -/
 theorem Var.weaken_rename_comm {x : Var k s1} {f : Rename s1 s2} :
@@ -135,8 +135,8 @@ inductive Exp.IsClosed : Exp s -> Prop where
     Exp.IsClosed (.abs cs T e)
 | tabs : CaptureSet.IsClosed cs -> PureTy.IsClosed T -> Exp.IsClosed e ->
     Exp.IsClosed (.tabs cs T e)
-| cabs : CaptureSet.IsClosed cs -> Exp.IsClosed e ->
-    Exp.IsClosed (.cabs cs m e)
+| cabs : CaptureSet.IsClosed cs -> CaptureBound.IsClosed cb -> Exp.IsClosed e ->
+    Exp.IsClosed (.cabs cs cb e)
 | boxed : CaptureSet.IsClosed cs -> SepCtx.IsClosed Ψ -> Exp.IsClosed e ->
     Exp.IsClosed (.boxed cs Ψ e)
 | reader : Var.IsClosed x -> Exp.IsClosed (.reader x)
